ref_impl/src/verifier/fstar_files/bosqueTypes.fst
@@ -37,9 +37,10 @@ type bosqueType =
 | BKeyedType
 | BErrorType
 // User-defined types
+| BnSMain__Baz2Type
 | BnSMain__Bar2Type
 | BnSMain__Bar3Type
-| BnSMain__Baz2Type
+| BnSMain__Baz3Type
 | BnSMain__MusicianType
 | BnSMain__ArtistType
 | BnSMain__PlayerMarkType
@@ -102,17 +103,19 @@ let rec subtypeOf x y = match x, y with
 // | BKeyedType, ? -> ?
 // User-defined types
 // Reflexivity relation
+| BnSMain__Baz2Type, BnSMain__Baz2Type -> true
 | BnSMain__Bar2Type, BnSMain__Bar2Type -> true
 | BnSMain__Bar3Type, BnSMain__Bar3Type -> true
-| BnSMain__Baz2Type, BnSMain__Baz2Type -> true
+| BnSMain__Baz3Type, BnSMain__Baz3Type -> true
 | BnSMain__MusicianType, BnSMain__MusicianType -> true
 | BnSMain__ArtistType, BnSMain__ArtistType -> true
 | BnSMain__PlayerMarkType, BnSMain__PlayerMarkType -> true
 // Provide relation
+| BnSMain__Baz2Type, BnSMain__Baz3Type -> true
 | BnSMain__Bar2Type, BnSMain__Baz2Type -> true
-| BObjectType, BnSMain__Bar2Type -> true
-| BObjectType, BnSMain__Bar3Type -> true
 | BnSMain__Bar3Type, BnSMain__Baz2Type -> true
+| BObjectType, BnSMain__Bar3Type -> true
+| BObjectType, BnSMain__Bar2Type -> true
 | BParsableType, BnSMain__MusicianType -> true
 | BParsableType, BnSMain__ArtistType -> true
 | BParsableType, BnSMain__PlayerMarkType -> true
